refactor and work on specs

VST-introduction/ASI_kalloc.v
@@ -20,12 +20,12 @@ Record KallocFreeAPD := {
   mem_mgr: globals -> mpred;
 }.
 
-Definition kalloc_token {cs:compspecs} M (sh: share) (t: type) (p: val): mpred := 
+Definition kalloc_token {cs:compspecs} K (sh: share) (t: type) (p: val): mpred := 
    !! field_compatible t [] p && 
-   kalloc_token' M sh (sizeof t) p.
+   kalloc_token' K sh (sizeof t) p.
 
-Lemma kalloc_token_valid_pointer: forall {cs: compspecs} M sh t p, 
-      kalloc_token M sh t p |-- valid_pointer p.
+Lemma kalloc_token_valid_pointer: forall {cs: compspecs} K sh t p, 
+      kalloc_token K sh t p |-- valid_pointer p.
 Proof. intros. unfold kalloc_token.
  apply andp_left2. apply kalloc_token'_valid_pointer.
 Qed.
@@ -33,8 +33,8 @@ Qed.
 #[export] Hint Resolve kalloc_token'_valid_pointer : valid_pointer.
 #[export] Hint Resolve kalloc_token_valid_pointer : valid_pointer.
 
-Lemma kalloc_token_local_facts:  forall {cs: compspecs} M sh t p,
-      kalloc_token M sh t p |-- !! (field_compatible t [] p /\ malloc_compatible (sizeof t) p).
+Lemma kalloc_token_local_facts:  forall {cs: compspecs} K sh t p,
+      kalloc_token K sh t p |-- !! (field_compatible t [] p /\ malloc_compatible (sizeof t) p).
 Proof. intros.
  unfold kalloc_token.
  normalize. rewrite prop_and.
@@ -46,23 +46,23 @@ Qed.
 #[export] Hint Resolve kalloc_token_local_facts : saturate_local.
 
 Section Kalloc_ASI.
-Variable M: KallocFreeAPD.
+Variable K: KallocFreeAPD.
 Variable kalloc1ID: ident.
 Variable kfree1ID: ident.
 
 Definition kalloc1_spec := 
-   DECLARE (*_malloc*)kalloc1ID
-   WITH n:Z, gv:globals
-   PRE [ size_t ]
-       PROP (0 <= n <= Ptrofs.max_unsigned(* - (WA+WORD)*))
-       PARAMS ((Vptrofs (Ptrofs.repr n))) GLOBALS (gv)
-       SEP ( mem_mgr M gv )
-   POST [ tptr tvoid ] EX p:_,
+   DECLARE (*_kalloc*)kalloc1ID
+   WITH n:Z, gv:globals, original_freelist_pointer:val
+   PRE [ ]
+       PROP (0 <= n <= Ptrofs.max_unsigned(* - (WA+WORD)*) /\ is_pointer_or_null original_freelist_pointer)
+       PARAMS () GLOBALS (gv)
+       SEP ( mem_mgr K gv )
+   POST [ tptr tvoid ]
        PROP ()
-       LOCAL (temp ret_temp p)
-       SEP ( mem_mgr M gv;
-             if eq_dec p nullval then emp
-             else (kalloc_token' M Ews n p * memory_block Ews n p)).
+       RETURN (original_freelist_pointer)
+       SEP ( mem_mgr K gv;
+             if eq_dec original_freelist_pointer nullval then emp
+             else (kalloc_token' K sh n original_freelist_pointer * memory_block sh n original_freelist_pointer)).
 
 Definition kfree1_spec :=
  DECLARE (*_kfree*)kfree1ID
@@ -70,13 +70,13 @@ Definition kfree1_spec :=
    PRE [ tptr tvoid ]
        PROP ()
        PARAMS (p) GLOBALS (gv)
-       SEP (mem_mgr M gv;
+       SEP (mem_mgr K gv;
             if eq_dec p nullval then emp
-            else (kalloc_token' M Ews n p * memory_block Ews n p))
+            else (kalloc_token' K sh n p * memory_block sh n p))
     POST [ Tvoid ]
        PROP ()
        LOCAL ()
-       SEP (mem_mgr M gv).
+       SEP (mem_mgr K gv).
 
 Definition Kalloc_ASI:funspecs := [kalloc1_spec; kfree1_spec].
 End Kalloc_ASI.
