VST-introduction/verif_client111111.v
@@ -8,76 +8,6 @@ Definition Vprog : varspecs. mk_varspecs prog. Defined.
 
 Local Open Scope logic.
 
-(************************ freelistrep *********************************)
-Fixpoint freelistrep (sh: share) (il: list val) (p: val) : mpred := (* the list contains the next*)
- match il with
- | next::il' =>
-        !! malloc_compatible (sizeof t_run) p &&  (* p is compatible with a memory block of size sizeof theader. *)
-        data_at sh t_run next p * (* at the location p, there is a t_run structure with the value next *)
-        freelistrep sh il' next (* "*" ensures no loops... *)
- | nil => !! (p = nullval) && emp
- end.
-
-Arguments freelistrep sh il p : simpl never.
-
-Ltac refold_freelistrep :=
-  unfold freelistrep;
-  fold freelistrep.
-
-Lemma freelistrep_local_prop: forall sh n p, 
-   freelistrep sh n p |--  !! (is_pointer_or_null p /\ (n=nil<->p=nullval) /\ ((n <> nil)<->isptr p))%nat.
-Proof.
-  intros.
-  induction n as [| n' IH].
-  - unfold freelistrep. entailer!. split; auto.
-    + split; auto.
-    + split; try lia. intros. simpl in *. auto_contradict. intros; auto_contradict.
-  - unfold freelistrep. destruct p; entailer!. split.
-    + split; intros; inversion H2.
-    + split; intros; auto. unfold not; intros. auto_contradict.
-   Qed.
-#[export] Hint Resolve freelistrep_local_prop : saturate_local.
-
-Lemma freelistrep_valid_pointer:
-  forall sh n p, 
-  readable_share sh ->
-   freelistrep sh n p |-- valid_pointer p.
-Proof.
-  intros. destruct n.
-  - unfold freelistrep. entailer!.
-  - unfold freelistrep. entailer.
-Qed. 
-#[export] Hint Resolve freelistrep_valid_pointer : valid_pointer.
-
-
-Lemma freelistrep_null: forall sh n x,
-       x = nullval ->
-       freelistrep sh n x = !! (n = nil) && emp.
-Proof.
-   intros.
-   destruct n; refold_freelistrep.
-   autorewrite with norm. auto.
-   apply pred_ext.
-   entailer. 
-   destruct n; entailer!; try discriminate H0. 
-Qed.
-
-Lemma freelistrep_nonnull: forall il sh x,
-   x <> nullval ->
-   freelistrep sh il x =
-   EX head : val, EX tail:list val,
-          !! (il = head::tail) && !! malloc_compatible (sizeof t_run) x && data_at sh t_run head x * freelistrep sh tail head.
-Proof.
-   intros; apply pred_ext.
-   - destruct il. 
-         + unfold freelistrep. entailer!.
-         + refold_freelistrep. entailer!.
-         Exists v il. 
-         entailer!. 
-   - Intros m y. rewrite H0. unfold freelistrep at 2; fold freelistrep. entailer!.
-Qed.
-
-
 
 
 (************************ specs *********************************)
@@ -434,7 +364,7 @@ Definition client9_spec :=
                     )
                 ).
 
-Definition client_11_pipealloc_spec := 
+(*Definition client_11_pipealloc_spec := 
     DECLARE _client_11_pipealloc
     WITH sh : share, original_freelist_pointer:val, xx:Z, ls:list val, gv:globals
     PRE [ ]
@@ -473,7 +403,7 @@ Definition client_11_pipealloc_spec :=
                     freelistrep sh ls' next *
                     data_at sh t_struct_kmem (Vint (Int.repr xx), next) (gv _kmem))
                 )                
-                ).
+                ).*)
 (* added values: 
 (pointers_with_original_head (Z.to_nat (n-1)) (pa1) PGSIZE original_freelist_pointer)
 *)
@@ -538,8 +468,8 @@ Definition Gprog : funspecs := [
     client5_spec;
     client6_spec;
     client7_spec;
-    client8_spec;
-    client_11_pipealloc_spec(*;
+    client8_spec
+    (*client_11_pipealloc_spec*)(*;
     freerange_while_loop_spec*)
 ].
 
