VST-introduction/VSU_kalloc_kfree_definitions.v
@@ -1,0 +1,62 @@
+Require Import VST.floyd.proofauto.
+Require Import VC.ASI_kalloc.
+Require Import VC.client1.
+Require Import VC.helper.
+(*Require Import malloc_lemmas.
+Require Import malloc_sep.*)
+
+(* THIS SHOULD CONTAIN ANY INTERNAL FUNCTIONS... I DON'T HAVE ANY *)
+
+
+Definition my_kalloc_token (sh: share) (sz: Z) (p: val) : mpred := (* my kalloc token is a block where we can have t_run struct in it, but also something else?*)
+  !! (field_compatible t_run [] p 
+      /\ malloc_compatible (sz) p
+      /\ 0 <= sizeof t_run <= sz
+      /\ writable_share sh) 
+ &&  memory_block sh (sz) (p). (* this is the rest of the page*)
+
+(** **** Exercise: 2 stars, standard (malloc_token_properties) *)
+Lemma my_kalloc_token_valid_pointer:
+    forall (sh : share) (sz : Z) (p : val),
+      my_kalloc_token sh sz p |-- valid_pointer p.
+Proof.
+  intros. 
+    induction sz.
+  - unfold my_kalloc_token. simpl. entailer!.
+  - unfold my_kalloc_token. simpl. entailer!.
+  - unfold my_kalloc_token. entailer!. 
+Qed.
+
+Lemma  my_kalloc_token_local_facts : 
+   forall (sh : share) (sz : Z) (p : val),
+     my_kalloc_token sh sz p |-- !! malloc_compatible sz p.
+Proof.
+  intros. 
+  unfold my_kalloc_token. simpl. entailer!.
+Qed.
+
+Definition Tok_APD := Build_KallocTokenAPD my_kalloc_token my_kalloc_token_valid_pointer
+   my_kalloc_token_local_facts.
+
+Definition mem_mgr (gv: globals) : mpred :=
+   EX sh: share, EX i: Z, EX p: val, EX ls: list val, EX xx, EX original_freelist_pointer,
+      data_at sh t_struct_kmem (Vint (Int.repr xx), original_freelist_pointer) (gv _kmem) *
+      freelistrep sh ls original_freelist_pointer.
+
+Definition KF_APD := Build_KallocFreeAPD Tok_APD mem_mgr.
+
+(*+ specs of private functions *)
+
+
+Definition MF_Vprog : varspecs. mk_varspecs prog. Defined.
+
+Definition MF_internal_specs: funspecs :=
+    [].
+   (*++ _malloc _free.*)
+
+(*Definition MF_Imports:funspecs := Mmap0_ASI _mmap0 _munmap.*)
+
+Definition MF_Gprog:funspecs := (*MF_Imports ++*) MF_internal_specs.
+(* I don't think I have any internal specs netiher MF imports..*)
+
+Ltac start_function_hint ::= idtac. (* no hint reminder *)
