VST-introduction/verif_kalloc1_kfree1.v
@@ -1,0 +1,22 @@
+Require Import VST.floyd.proofauto.
+Require Import VC.ASI_kalloc.
+Require Import VC.client1.
+Require Import VC.helper.
+
+#[export] Instance CompSpecs : compspecs. make_compspecs prog. Defined.
+Definition Vprog : varspecs. mk_varspecs prog. Defined.
+
+Local Open Scope logic.
+
+(*Require Import malloc.
+Require Import malloc_lemmas.
+Require Import malloc_sep.*)
+Require Import VC.VSU_kalloc_kfree_definitions.
+
+Lemma body_kfree1 i: semax_body MF_Vprog MF_Gprog f_kfree1 (kfree1_spec KF_APD i).
+Proof. start_function.
+Admitted.
+
+Lemma body_kalloc1 i: semax_body MF_Vprog MF_Gprog f_kalloc1 (kalloc1_spec KF_APD i).
+Proof. start_function. 
+Admitted.
